In the process of proving proposition 4.17 (the if part)

Forkable_Strings.thy
@@ -1,4 +1,4 @@
-theory Forkable_Strings imports Main "~~/src/HOL/List" begin
+theory Forkable_Strings imports Main "~~/src/HOL/List" "~~/src/HOL/Finite_Set" begin
 
 text "We will use True as 1 and False as 0 in characteristic strings; we might think about each bool
 value answers to the question 'is this slot controlled by an adversarial player?'."
@@ -122,7 +122,35 @@ lemma Listmax_ge [simp]: "\<forall>x \<in> set l. x \<le> ListMax l"
     then show ?case
       using Cons.IH by auto 
   qed
-    
+
+lemma ListMax_member [simp]: "l = [] \<or> (\<exists> x \<in> set l. ListMax l = x)"   
+  proof (induction l)
+    case Nil
+    then show ?case by simp
+  next
+    case (Cons a l)
+    have "a#l \<noteq> []" by simp
+    then show ?case 
+    proof (cases "l = []")
+      case True
+      then have "ListMax (a#l) = max a (foldr max l 0)"
+        by (metis ListMax_def foldr.simps(2) o_def)
+      hence "ListMax (a#l) = a"
+        by (metis ListMax_0 ListMax_def True max_0R)
+      then show ?thesis
+        by (metis list.set_intros(1)) 
+    next
+      case False
+        then have "ListMax (a#l) = max a (foldr max l 0)"
+        by (metis ListMax_def foldr.simps(2) o_def)
+      hence "ListMax (a#l) = ListMax l \<or> ListMax (a#l) = a"
+        by (metis ListMax_def max_def)
+      then show ?thesis
+        by (metis Cons.IH False insert_iff list.set(2)) 
+    qed
+      
+  qed
+ 
 fun height :: "nattree \<Rightarrow> nat" where
   "height Empty = 0"  
 | "height (Node n bl) = (if Leaf (Node n bl) then 0 else Suc (ListMax (map height bl)))"
@@ -217,31 +245,48 @@ fun maxOption :: "nat option \<Rightarrow> nat option \<Rightarrow> nat option" 
   
 definition ListMaxOption :: "(nat option) list \<Rightarrow> nat option" where
   "ListMaxOption l = foldr maxOption l None"
-
+                                             
+lemma ListMaxOption_none_imp_all_none [simp]: "ListMaxOption l = None \<longleftrightarrow> (\<forall>x \<in> set l. x = None)" 
+proof (induction l)
+  case Nil
+    hence "ListMaxOption [] =  None"
+      by (simp add: ListMaxOption_def)
+  then show ?case
+    by simp 
+  next
+    case (Cons y ys)
+      hence "ListMaxOption (y#ys) = maxOption y (foldr maxOption ys None)"
+        by (simp add: ListMaxOption_def)
+      hence "ListMaxOption (y#ys) = None \<longrightarrow> y = None \<and> (foldr maxOption ys None) = None"
+        by (metis (no_types, lifting) maxOption.elims option.case_eq_if option.simps(3))
+    then show ?case
+      using Cons.IH ListMaxOption_def by force 
+  qed
+                                   
 definition SucOption :: "nat option \<Rightarrow> nat option" where
   "SucOption n = (case n of None \<Rightarrow> None | Some n \<Rightarrow> Some (Suc n))"
-  
-fun le_option :: "nat option \<Rightarrow> nat option \<Rightarrow> bool" where  
-  "le_option None _ = True"
-| "le_option (Some n) x = (case x of None \<Rightarrow> False | Some m \<Rightarrow> n \<le> m)"
 
+lemma SucOption_none [simp]: "SucOption x = None \<longrightarrow> x = None"
+  by (simp add: SucOption_def option.case_eq_if)  
+  
 text "We don't care None cases"
-fun lt_option :: "nat option \<Rightarrow> nat option \<Rightarrow> bool" where
-  "lt_option None _ = False" 
-| "lt_option _ None = False"  
-| "lt_option (Some m) (Some n) = (m < n)"
+inductive lt_option :: "nat option \<Rightarrow> nat option \<Rightarrow> bool" where
+"m < n \<Longrightarrow> lt_option (Some m) (Some n)"  
  
+inductive le_option :: "nat option \<Rightarrow> nat option \<Rightarrow> bool" where
+"m \<le> n \<Longrightarrow> le_option (Some m) (Some n)"
+
 fun depth :: "nattree \<Rightarrow> nat \<Rightarrow> nat option" where
   "depth Empty n = None"
 | "depth (Node n bl) m = (if n = m 
                           then (Some 0) 
                           else SucOption (ListMaxOption (map (\<lambda>x. depth x m) bl)))"
-
+  
 definition H :: "bool list \<Rightarrow> nat set" where
   "H l = {x. x \<le> length l \<and> \<not> (nth (False#l) x)}"
 
 definition isHonest :: "bool list \<Rightarrow> nat \<Rightarrow> bool" where
-  "isHonest l x = (\<not> (nth (False#l) x))"
+  "isHonest l x = (x \<in> H l)"
   
 lemma H_0 [simp]: "0 \<in> H l"
   by (simp add: H_def)
@@ -253,7 +298,7 @@ lemma getFrom_suc_eq_H [simp]: "x < length l \<and> \<not> nth l x \<longleftrig
 fun ListSum :: "nat list \<Rightarrow> nat" where
   "ListSum l = foldr plus l 0"
 
-lemma ListSum_0 [simp] :"(\<forall>x \<in> set l. x = 0) \<longrightarrow> ListSum l = 0" 
+lemma ListSum_0 [simp] :"(\<forall>x \<in> set l. x = 0) \<longleftrightarrow> ListSum l = 0" 
   proof (induction l)
     case Nil
     then show ?case by simp
@@ -262,8 +307,20 @@ lemma ListSum_0 [simp] :"(\<forall>x \<in> set l. x = 0) \<longrightarrow> ListS
     then show ?case
       by simp 
   qed
+    
+lemma ListSum_ge [simp] : "\<forall>x \<in> set l. ListSum l \<ge> x"
+  proof (induction l)
+    case Nil
+    then show ?case by simp
+  next
+    case (Cons x xs)
+      hence "ListSum (x#xs) = x + ListSum xs"
+        by simp
+      hence "ListSum (x#xs) \<ge> x" by simp
+    then show ?case using Cons.IH by auto
+  qed
+    
 text "No prunning used as we don't yet have an increasing tree in argument, but can improve it later"
-
 fun count_node :: "nat \<Rightarrow> nattree \<Rightarrow> nat" where
   "count_node _ Empty = 0"
 | "count_node m (Node n bl) = (of_bool (m = n)) + ListSum (map (count_node m) bl)"
@@ -317,7 +374,7 @@ lemma max_node_max [simp]: "\<forall> m. max_node t < m  \<longrightarrow> count
       by (smt Listmax_ge a add.commute add_cancel_left_right count_node.simps(2) list.set_intros(1) 
           not_le of_bool_def)
       then show ?case
-      using ListSum_0 \<open>\<forall>x. \<forall>y\<in>set x2. max_node (Node x1 x2) < x \<longrightarrow> count_node x y = 0\<close> by auto 
+        by (metis (full_types) ListSum_0 Listmax_ge \<open>\<forall>x. \<forall>y\<in>set x2. max_node (Node x1 x2) < x \<longrightarrow> count_node x y = 0\<close> le_zero_eq listmax_0)
   qed
   
 fun increasing_depth_H :: "nattree \<Rightarrow> bool list \<Rightarrow> bool" where 
@@ -357,13 +414,303 @@ fun getLabelFromTine :: "nattree \<Rightarrow> nat list \<Rightarrow> nat list" 
 | "getLabelFromTine (Node _ l) (x#xs) = (if x \<ge> length l then [] else 
                                            (case nth l x of 
                                             Empty \<Rightarrow> [] | (*it runs out of nodes before we can trace down all paths*)
-                                            Node n _ \<Rightarrow> n # getLabelFromTine (hd (drop x l)) xs))"  
+                                            Node n _ \<Rightarrow> n # getLabelFromTine (nth l x) xs))"  
 
 text "This function provides a set of all path possible, starting from a root by comparing between
 the length of lists of all choices of edges and lists of their labels."
 fun set_of_tines :: "nattree \<Rightarrow> (nat list) set" where
   "set_of_tines t  = {tine. length tine = length (getLabelFromTine t tine)}"  
+  
+lemma getLabelFromTine_Leaf_nil : assumes "Leaf F" shows "getLabelFromTine F t = []"
+proof -
+  obtain l and n where "ListOfEmpty l \<and> F = Node n l"
+    using Leaf.cases assms by blast
+  thus ?thesis 
+   proof (cases t)
+     case Nil
+     then show ?thesis
+       by (simp add: \<open>ListOfEmpty l \<and> F = Node n l\<close>) 
+   next
+     case (Cons x xs)
+     then show ?thesis 
+       proof (cases "x \<ge> length l")
+         case True
+         then show ?thesis
+           by (simp add: \<open>ListOfEmpty l \<and> F = Node n l\<close> local.Cons) 
+       next
+         case False
+         then show ?thesis
+           by (metis Leaf_non_ListOfEmpty \<open>ListOfEmpty l \<and> F = Node n l\<close> assms eq_iff 
+getLabelFromTine.simps(3) less_imp_le_nat linorder_neqE_nat local.Cons nattree.simps(4) nth_mem)
+       qed
+   qed
+ qed
+   
+lemma getLabelFromTine_shorter_eq_height [simp]: "length (getLabelFromTine F t) \<le> height F"
+proof (induction t arbitrary:F)
+     case Nil
+     then show ?case
+       by (metis getLabelFromTine.elims getLabelFromTine.simps(2) less_eq_nat.simps(1) list.size(3))
+   next
+     case (Cons x xs)
+     then show ?case 
+       proof (induction F)
+         case Empty
+         then show ?case by simp
+       next
+         case (Node n l)
+           have "getLabelFromTine (Node n l) (x#xs) = (if x \<ge> length l then [] else 
+                                           (case nth l x of 
+                                            Empty \<Rightarrow> [] | (*it runs out of nodes before we can trace down all paths*)
+                                            Node m _ \<Rightarrow> m # getLabelFromTine (nth l x) xs))" using getLabelFromTine.simps(3) by simp
+           then show ?case 
+             proof (cases "x \<ge> length l")
+               case True
+               then show ?thesis
+                 by (metis getLabelFromTine.simps(3) le0 list.size(3)) 
+             next
+               case False
+               then show ?thesis 
+                 proof (cases "nth l x")
+                   case Empty
+                   then show ?thesis
+                     by (metis \<open>getLabelFromTine (Node n l) (x # xs) = (if length l \<le> x then [] else 
+case l ! x of Empty \<Rightarrow> [] | Node m xa \<Rightarrow> m # getLabelFromTine (l ! x) xs)\<close> le0 list.size(3) nattree.simps(4)) 
+                 next
+                   case (Node m bl)
+                     hence "getLabelFromTine (Node n l) (x#xs) = m # getLabelFromTine (nth l x) xs"
+                       by (simp add: False)
+                     hence "length (getLabelFromTine (Node n l) (x#xs)) = Suc (length (getLabelFromTine (nth l x) xs))"
+                       by simp
+                     hence "length (getLabelFromTine (nth l x) xs) \<le> height (nth l x)"
+                       by (simp add: Node.prems)
+                     hence  "length (getLabelFromTine (Node n l) (x#xs)) \<le> Suc (height (nth l x))"
+                       using \<open>length (getLabelFromTine (Node n l) (x # xs)) = Suc (length (getLabelFromTine (l ! x) xs))\<close> by linarith
+                     have "Suc (height (nth l x)) \<le> height (Node n l)"
+                       by (metis (no_types, lifting) False Listmax_ge \<open>getLabelFromTine (Node n l) (x # xs) = m # getLabelFromTine (l ! x) xs\<close> getLabelFromTine_Leaf_nil height.simps(2) image_eqI linorder_not_le list.distinct(1) not_less_eq_eq nth_mem set_map)
+                     then show ?thesis
+                       using \<open>length (getLabelFromTine (Node n l) (x # xs)) \<le> Suc (height (l ! x))\<close> le_trans by blast 
+                 qed
+             qed
+       qed
+ qed
+        
 
+      
+lemma getLabelFromTine_shorter_eq_tine [simp]: "length (getLabelFromTine F t) \<le> length t"
+  sorry
+    
+lemma set_of_tines_Empty [simp]: "set_of_tines Empty = {[]}"
+  by simp
+   
+lemma getLabelFromTine_branch_notin [simp]: "x \<ge> length l \<longrightarrow> x#xs \<notin> set_of_tines (Node n l)"
+  by simp
+  
+lemma getLabelFromTine_branch_in_if [simp]: assumes "x < length l \<and> xs \<in> set_of_tines (nth l x) \<and> (nth l x \<noteq> Empty)" shows "x#xs \<in> set_of_tines (Node n l)"
+proof (cases "nth l x")
+  case Empty
+  then show ?thesis
+    using assms by auto
+next
+  case (Node m bl)
+  have "getLabelFromTine (Node n l) (x#xs) = m # getLabelFromTine (nth l x) xs"
+    using Node assms by auto
+  hence "length (getLabelFromTine (nth l x) xs) = length xs"
+    using assms by auto
+  then show ?thesis
+    using \<open>getLabelFromTine (Node n l) (x # xs) = m # getLabelFromTine (l ! x) xs\<close> by auto 
+qed
+
+lemma getLabelFromTine_branch_in_onlyif [simp]: assumes "x#xs \<in> set_of_tines (Node n l)" shows "x < length l \<and> xs \<in> set_of_tines (nth l x) \<and> (nth l x \<noteq> Empty)"  
+proof -
+  have "length (x#xs) = length (getLabelFromTine (Node n l) (x#xs))"
+    using assms by auto
+  have len:"x < length l"
+  proof -
+    have "\<not> length l \<le> x"
+      by (metis assms getLabelFromTine_branch_notin)
+    then show ?thesis
+      by auto
+  qed
+  have empty:"nth l x \<noteq> Empty"
+    by (metis \<open>length (x # xs) = length (getLabelFromTine (Node n l) (x # xs))\<close> assms 
+getLabelFromTine.simps(3) getLabelFromTine_branch_notin length_0_conv list.simps(3) nattree.simps(4))
+  then obtain m bl where "nth l x = Node m bl" using len
+    using max_node.cases by blast
+  hence "getLabelFromTine (Node n l) (x#xs) = m # getLabelFromTine (nth l x) xs" using len empty
+    by simp
+  thus ?thesis
+    using \<open>length (x # xs) = length (getLabelFromTine (Node n l) (x # xs))\<close> len by auto
+qed
+
+lemma getLabelFromTine_branch_in [simp]: "x#xs \<in> set_of_tines (Node n l) \<longleftrightarrow> x < length l \<and> xs \<in> set_of_tines (nth l x) \<and> (nth l x \<noteq> Empty)"
+  using getLabelFromTine_branch_in_if getLabelFromTine_branch_in_onlyif by blast
+  
+lemma nil_in_set_of_tines [simp]: "[] \<in> set_of_tines F"  
+  by (metis (mono_tags) getLabelFromTine.simps(1) getLabelFromTine.simps(2) length_0_conv list.size(3) 
+mem_Collect_eq nattree.exhaust set_of_tines.simps) 
+
+lemma nth_in_fst [simp] : assumes "n < length x" shows "nth x n = nth (x@y) n"
+  by (simp add: assms nth_append)
+
+lemma finite_set_of_tines_aux_0_aux [simp]: "getLabelFromTine (Node n (xs@[Empty])) t = getLabelFromTine (Node n xs) t"
+proof (cases t)
+  case Nil
+  then show ?thesis by simp
+next
+  case (Cons y ys)
+  then show ?thesis 
+    proof (cases "y \<ge> length (xs@[Empty])")
+      case True
+      hence L:"getLabelFromTine (Node n (xs@[Empty])) (y#ys) = []"
+        by simp
+      have R:"getLabelFromTine (Node n xs) (y#ys) = []" using True  by simp
+      then show ?thesis using L
+        by (simp add: local.Cons)  
+    next
+      case False
+        hence lt1:"y < length (xs@[Empty])"
+          by simp
+      then show ?thesis 
+        proof (cases "y = length xs")
+          case True
+          then show ?thesis
+            by (simp add: local.Cons) 
+        next
+          case False
+            hence  lt2:"y < length xs"
+              using \<open>y < length (xs @ [Empty])\<close> by auto
+            hence nth_eq:"nth xs y = nth (xs@[Empty]) y"
+              by simp
+            hence L:"getLabelFromTine (Node n (xs@[Empty])) (y#ys) =  
+                                            (case nth (xs@[Empty]) y of 
+                                            Empty \<Rightarrow> [] | 
+                                            Node m _ \<Rightarrow> m # getLabelFromTine (nth (xs@[Empty]) y) ys)" using lt1 by simp
+            have R:"getLabelFromTine (Node n xs) (y#ys) =  
+                                            (case nth xs y of 
+                                            Empty \<Rightarrow> [] | 
+                                            Node m _ \<Rightarrow> m # getLabelFromTine (nth xs y) ys)" using lt2 by simp
+          then show ?thesis using L R nth_eq
+            using local.Cons by presburger
+        qed
+    qed
+qed
+  
+lemma finite_set_of_tines_aux_0 [simp]: "set_of_tines (Node n (xs@[Empty])) = set_of_tines (Node n xs)"
+proof -
+  have "set_of_tines (Node n (xs@[Empty])) = {tine. length tine = length (getLabelFromTine (Node n (xs@[Empty])) tine)}"
+    by auto
+  hence "set_of_tines (Node n (xs@[Empty])) = {tine. length tine = length (getLabelFromTine (Node n xs) tine)}"
+    by auto
+  thus ?thesis
+    by simp
+qed   
+
+lemma finite_set_of_tines_aux_1_aux [simp]: "length y = length (getLabelFromTine (Node n (xs@[Node m l])) y) 
+       \<longrightarrow> y \<in> set_of_tines (Node n xs) \<or> y \<in> {r. \<exists>s \<in> set_of_tines (Node m l). r = (length xs)#s}"
+proof (cases y)
+  case Nil
+  then show ?thesis
+    by simp 
+next
+  case (Cons y ys)
+    have "\<forall>y ys. y < length xs \<longrightarrow> getLabelFromTine (Node n (xs@[Node m l])) (y#ys) = (case nth (xs@[Node m l]) y of 
+                                                                                          Empty \<Rightarrow> [] | 
+                                                                                          Node p _ \<Rightarrow> p # getLabelFromTine (nth (xs@[Node m l]) y) ys)" 
+    by auto
+  hence "\<forall>y ys. y < length xs \<longrightarrow> getLabelFromTine (Node n (xs@[Node m l])) (y#ys) = (case nth xs y of 
+                                                                                          Empty \<Rightarrow> [] | 
+                                                                                          Node p _ \<Rightarrow> p # getLabelFromTine (nth xs y) ys)"
+    by (metis nth_in_fst)
+     hence lt:"\<forall>y ys. y < length xs \<longrightarrow> getLabelFromTine (Node n (xs@[Node m l])) (y#ys) = getLabelFromTine (Node n xs) (y#ys)"
+       by simp
+   have cons:"\<forall>y ys. length (y#ys) = length (getLabelFromTine (Node n (xs@[Node m l])) (y#ys)) 
+       \<longrightarrow> (y#ys) \<in> set_of_tines (Node n xs) \<or> (y#ys) \<in> {r. \<exists>s \<in> set_of_tines (Node m l). r = (length xs)#s}"
+    using Suc_le_eq length_Cons lt by auto 
+  then show ?thesis
+    using local.Cons by blast 
+qed
+  
+lemma finite_set_of_tines_aux_1 [simp]: "set_of_tines (Node n (xs@[Node m l])) = set_of_tines (Node n xs) \<union> {r. \<exists>s \<in> set_of_tines (Node m l). r = (length xs)#s}"
+proof -
+  have "\<forall>y ys. y < length xs \<longrightarrow> getLabelFromTine (Node n (xs@[Node m l])) (y#ys) = (case nth (xs@[Node m l]) y of 
+                                                                                          Empty \<Rightarrow> [] | 
+                                                                                          Node p _ \<Rightarrow> p # getLabelFromTine (nth (xs@[Node m l]) y) ys)" 
+    by auto
+  hence "\<forall>y ys. y < length xs \<longrightarrow> getLabelFromTine (Node n (xs@[Node m l])) (y#ys) = (case nth xs y of 
+                                                                                          Empty \<Rightarrow> [] | 
+                                                                                          Node p _ \<Rightarrow> p # getLabelFromTine (nth xs y) ys)"
+    by (metis nth_in_fst)
+  hence lt:"\<forall>y ys. y < length xs \<longrightarrow> getLabelFromTine (Node n (xs@[Node m l])) (y#ys) = getLabelFromTine (Node n xs) (y#ys)"
+    by simp  
+  have "\<forall>x \<in> set_of_tines (Node n (xs@[Node m l])). x \<in> set_of_tines (Node n xs) \<union> {r. \<exists>s \<in> set_of_tines (Node m l). r = (length xs)#s}"
+    using finite_set_of_tines_aux_1_aux by auto
+  hence "set_of_tines (Node n (xs@[Node m l])) \<subseteq> set_of_tines (Node n xs) \<union> {r. \<exists>s \<in> set_of_tines (Node m l). r = (length xs)#s}"
+    by blast 
+  have cons:"\<forall>y ys. length (y#ys) = length (getLabelFromTine (Node n xs) (y#ys)) 
+       \<longrightarrow> (y#ys) \<in> set_of_tines (Node n (xs@[Node m l]))"
+    using lt by auto
+  hence "\<forall>x. length x = length (getLabelFromTine (Node n xs) x) \<longrightarrow> x \<in> set_of_tines (Node n (xs@[Node m l]))"
+    by (metis list.exhaust nil_in_set_of_tines) 
+  hence main: "\<forall>x \<in> set_of_tines (Node n xs). x \<in> set_of_tines (Node n (xs@[Node m l]))"
+    by simp
+  have "\<forall>x \<in> {r. \<exists>s \<in> set_of_tines (Node m l). r = (length xs)#s}. x \<in> set_of_tines (Node n (xs@[Node m l]))"
+    by auto
+  hence "set_of_tines (Node n xs) \<union> {r. \<exists>s \<in> set_of_tines (Node m l). r = (length xs)#s} \<subseteq> set_of_tines (Node n (xs@[Node m l]))" using main
+    by blast
+    then show ?thesis
+      using \<open>set_of_tines (Node n (xs @ [Node m l])) \<subseteq> set_of_tines (Node n xs) \<union> {r. \<exists>s\<in>set_of_tines (Node m l). r = length xs # s}\<close> by blast   
+qed
+
+lemma finite_cons [simp]: assumes "finite x" shows "finite {r. \<exists>s \<in> x. r = m # s}"  
+proof -
+  have "{r. \<exists>s \<in> x. r = m # s} = (\<lambda>s. m#s)`x"
+    by (simp add: image_def)
+  thus ?thesis
+    by (simp add: assms)
+qed
+  
+lemma finite_set_of_tines [simp]: "finite (set_of_tines t)"
+  proof (induction t)
+    case Empty
+    then show ?case
+      by auto 
+  next
+    case (Node n l)
+    then show ?case 
+      proof (induct l rule: rev_induct)
+        case Nil
+          hence "set_of_tines (Node n []) = {tine. length tine = length (getLabelFromTine (Node n []) tine)}"
+            by simp
+          hence "set_of_tines (Node n []) = {tine. length tine = 0}"
+            by (metis (no_types, lifting) Collect_cong Leaf.intros ListOfEmpty.Nil getLabelFromTine_Leaf_nil list.size(3))
+          hence "set_of_tines (Node n []) = {[]}"
+            by auto
+          then show ?case
+            by simp 
+      next
+        case (snoc x xs)
+        then have "finite (set_of_tines x) \<and> ((\<forall>y \<in> set xs. finite (set_of_tines y)) \<longrightarrow> finite (set_of_tines (Node n xs)))" by simp 
+        hence "(\<forall>y \<in> set xs. finite (set_of_tines y)) \<longrightarrow> finite (set_of_tines (Node n (xs@[x])))"
+          proof (cases x)
+            case Empty
+            then show ?thesis 
+              using snoc.hyps snoc.prems by auto  
+          next
+            case (Node m l)
+            hence "finite (set_of_tines (Node m l))"
+              using \<open>finite (set_of_tines x) \<and> ((\<forall>y\<in>set xs. finite (set_of_tines y)) \<longrightarrow> finite (set_of_tines (Node n xs)))\<close> 
+              by blast
+            hence "finite {r. \<exists>s\<in>set_of_tines (Node m l). r = length xs # s}"
+              by simp 
+            then show ?thesis
+              using Node finite_set_of_tines_aux_1 snoc.hyps by auto 
+          qed
+        then show ?case
+          using finite_set_of_tines_aux_1 finite_set_of_tines_aux_0 snoc.prems by auto
+      qed
+  qed
+  
 fun edge_disjoint_tines :: "nat list \<Rightarrow> nat list \<Rightarrow> bool" where
   "edge_disjoint_tines [] _ = True" 
 | "edge_disjoint_tines _ [] = True"
@@ -642,10 +989,30 @@ proof -
  qed
    
 definition set_of_edge_disjoint_tines :: "nattree \<Rightarrow> ((nat list, nat list) prod) set" where
- "set_of_edge_disjoint_tines t
+ "set_of_edge_disjoint_tines t         
    = {(x,y). x \<in> set_of_tines t 
       \<and> y \<in> set_of_tines t
       \<and> edge_disjoint_tines x y}" 
+
+lemma set_of_edge_disjoint_tines_finite : "finite (set_of_edge_disjoint_tines F)"
+proof -
+  have f1:"set_of_edge_disjoint_tines F = {(x,y). x \<in> set_of_tines F  \<and> y \<in> set_of_tines F \<and> edge_disjoint_tines x y}"
+    by (simp add: set_of_edge_disjoint_tines_def) 
+  have f2:"finite (set_of_tines F)"
+    using finite_set_of_tines by auto
+  hence "finite ((set_of_tines F) \<times> (set_of_tines F))"
+    by auto
+  hence "\<forall>a. fst a \<in> set_of_tines F  \<and> snd a \<in> set_of_tines F \<and> edge_disjoint_tines (fst a) (snd a) \<longrightarrow>  fst a \<in> set_of_tines F  \<and> (snd a) \<in> set_of_tines F"
+    by simp
+  hence "{(x,y). x \<in> set_of_tines F  \<and> y \<in> set_of_tines F \<and> edge_disjoint_tines x y} \<subseteq> {(x,y). x \<in> set_of_tines F  \<and> y \<in> set_of_tines F}"
+    by blast 
+  have "set_of_tines F \<times> set_of_tines F =  {(x,y). x \<in> set_of_tines F  \<and> y \<in> set_of_tines F}"
+    by blast
+  hence "finite {(x,y). x \<in> set_of_tines F  \<and> y \<in> set_of_tines F}"
+    using \<open>finite (set_of_tines F \<times> set_of_tines F)\<close> by auto
+  thus ?thesis
+    using \<open>{(x, y). x \<in> set_of_tines F \<and> y \<in> set_of_tines F \<and> edge_disjoint_tines x y} \<subseteq> {(x, y). x \<in> set_of_tines F \<and> y \<in> set_of_tines F}\<close> f1 infinite_super by auto 
+  qed
     
 definition margin :: "nattree \<Rightarrow>  bool list \<Rightarrow> int" where
   "margin t w = Max {r. (\<exists> (a,b) \<in> set_of_edge_disjoint_tines t. r = min (reach t w a) (reach t w b))}"
@@ -712,8 +1079,55 @@ fun remove_greater :: "nat \<Rightarrow> nattree \<Rightarrow> nattree" where
   | "remove_greater m (Node n l) = (if n < m then Node n (map (remove_greater m) l) else Empty)"
 
 definition max_honest_node :: "bool list \<Rightarrow> nat" where
-  "max_honest_node w = Max {r. r \<in> H w}"
+  "max_honest_node w = Max (H w)"
    
+lemma finite_honest_node [simp]: "finite (H w)"
+  proof (induct w rule: rev_induct)
+    case Nil
+    then show ?case
+      by simp 
+  next
+    case (snoc w ws)
+    have ws:"H ws = {x. x \<le> length ws \<and> \<not> (nth (False#ws) x)}"
+      by (simp add: H_def)
+    have ws_w : "H (ws@[w]) = {x. x \<le> length (ws@[w]) \<and> \<not> (nth (False#(ws@[w])) x)}"
+      by (simp add: H_def) 
+    hence imp:"\<forall>x. x \<le> length ws \<longrightarrow> (nth (False#ws) x =  nth (False#(ws@[w])) x)"
+      by (metis (full_types) Cons_eq_appendI le_imp_less_Suc length_Cons nth_in_fst)
+    hence "H (ws@[w]) = (if w then H ws else insert (length (ws@[w])) (H ws))"
+    proof (cases w)
+      case True
+        hence "nth (False#(ws@[w])) (length (ws@[w]))"
+          by simp
+      then show ?thesis using ws ws_w
+        by (smt Collect_cong Cons_eq_appendI True eq_iff le_imp_less_Suc length_Cons length_append_singleton nat_less_le not_less_eq_eq nth_in_fst)
+      next
+        case False
+        hence "\<not> nth (False#(ws@[w])) (length (ws@[w]))"
+          by simp
+         hence "length (ws@[w]) \<in> H (ws@[w])"
+           by (metis (no_types, lifting) eq_iff mem_Collect_eq ws_w)
+         hence "H (ws@[w]) = {x. x= length (ws@[w]) \<or> (x \<le> length ws \<and> \<not> (nth (False#(ws@[w])) x))}" using ws_w
+           by (smt Collect_cong False Suc_leD antisym dual_order.trans length_append_singleton mem_Collect_eq not_less_eq_eq)
+         hence "H (ws@[w]) = {x. x= length (ws@[w]) \<or> x \<in> {x. x \<le> length ws \<and> \<not> (nth (False#ws) x)}}"
+           by (smt Collect_cong imp mem_Collect_eq)
+         then show ?thesis
+           by (metis False insert_compr ws) 
+    qed
+    then show ?case
+      by (metis finite_insert snoc.hyps) 
+  qed 
+  
+lemma max_honest_node_le_length [simp]: "max_honest_node w \<le> length w"
+proof -
+  have "0 \<in> H w"
+    using H_0 by blast
+  have "\<forall>x \<in> H w. x \<le> length w"
+    by (simp add: H_def)
+  then show ?thesis using finite_honest_node
+    by (metis Max_in \<open>0 \<in> H w\<close> equals0D max_honest_node_def) 
+qed
+  
 fun count_node_by_set :: "nat set \<Rightarrow> nattree \<Rightarrow> nat" where
   "count_node_by_set _ Empty = 0"
 | "count_node_by_set s (Node n l) = (of_bool (n \<in> s)) +  ListSum (map (count_node_by_set s) l)"  
@@ -726,42 +1140,789 @@ lemma map_ListOfEmpty [simp]: "ListOfEmpty (map (\<lambda>x. Empty) l)"
   apply (simp add: ListOfEmpty.Nil)
   by (simp add: ListOfEmpty.Cons)
   
-(*This definition makes me reconsider the definition of prefixes of tines and forks.*)
 fun toClosedFork :: "bool list \<Rightarrow> nattree \<Rightarrow> nattree" where
   "toClosedFork _ Empty = Empty"
-| "toClosedFork w (Node n l) =
-(if  count_honest_node w (Node n l) = of_bool (isHonest w n)
+| "toClosedFork w (Node n l) = 
+(if count_honest_node w (Node n l) = of_bool (isHonest w n) (*0 or 1 *)
   then 
-    (if isHonest w n then Node n (map (\<lambda>x. Empty) l) else Empty)
-  else Node n (map (toClosedFork w) l)
-)"
+    (if isHonest w n 
+    then Node n (map (\<lambda>x. Empty) l)
+    else  Empty)
+  else Node n (map (toClosedFork w) l))"
 
+lemma isFork_toClosedFork_isFork_aux_1 [simp]: 
+ "length w \<ge> max_node F \<longrightarrow> length w \<ge> max_node (toClosedFork w F)"
+proof (induction F)
+  case Empty
+  then show ?case by simp
+next
+  case (Node n l)    
+    have "n \<le> max_node (Node n l)"
+      by simp
+  then show ?case 
+    proof (cases "count_honest_node w (Node n l) = of_bool (isHonest w n)")
+      case True
+      then have "count_honest_node w (Node n l) = of_bool (isHonest w n)" by simp
+      then show ?thesis 
+        proof (cases "isHonest w n")
+          case True (*solve this ambiguity*)
+          then show ?thesis
+            by (metis Leaf.intros \<open>count_honest_node w (Node n l) = of_bool (isHonest w n)\<close> 
+\<open>n \<le> max_node (Node n l)\<close> dual_order.trans map_ListOfEmpty max_node_Leaf toClosedFork.simps(2)) 
+        next 
+          case False
+          then have "toClosedFork w (Node n l) = Empty"
+            by (metis True toClosedFork.simps(2))
+          then show ?thesis
+            by (metis le_0_eq linear max_node.simps(1))
+      qed 
+     next
+      case False
+        then have "toClosedFork w (Node n l) = Node n (map (toClosedFork w) l)"
+          by simp
+        hence "max_node (toClosedFork w (Node n l)) 
+=  ListMax (n # (map max_node (map (toClosedFork w) l)))"
+          by simp
+        have f1 :"length w \<ge> max_node (Node n l) \<longrightarrow> length w \<ge> n"
+          by (metis \<open>n \<le> max_node (Node n l)\<close> le_trans)
+        have "length w \<ge> max_node (Node n l) \<longrightarrow> (\<forall> x \<in> set l. length w \<ge> max_node x)"
+          by (metis Listmax_ge dual_order.trans image_eqI insertCI list.set(2) max_node.simps(2) set_map)  
+        hence "length w \<ge> max_node (Node n l) \<longrightarrow> (\<forall> x \<in> set l. length w \<ge> max_node (toClosedFork w x))"
+          by (metis Node.IH)            
+        hence "l = [] \<or> (\<exists>x \<in> set (map max_node (map (toClosedFork w) l)). x = ListMax (map max_node (map (toClosedFork w) l)))"
+          using ListMax_member 
+          by (metis length_0_conv length_map) 
+        hence "l = [] \<or> (\<exists>x \<in> set (map (toClosedFork w) l). max_node x = ListMax (map max_node (map (toClosedFork w) l)))"
+          by (metis imageE set_map)
+        hence "l = [] \<or> (\<exists>x \<in> set l. max_node (toClosedFork w x) = ListMax (map max_node (map (toClosedFork w) l)))"
+          by (metis imageE set_map)
+        then show ?thesis
+          by (metis ListMax_member Listmax_ge 
+\<open>max_node (Node n l) \<le> length w \<longrightarrow> (\<forall>x\<in>set l. max_node (toClosedFork w x) \<le> length w)\<close> 
+\<open>max_node (toClosedFork w (Node n l)) = ListMax (n # map max_node (map (toClosedFork w) l))\<close> 
+\<open>toClosedFork w (Node n l) = Node n (map (toClosedFork w) l)\<close> dual_order.trans f1 list.discI list.simps(8) set_ConsD)             
+    qed    
+  qed
+
+lemma isFork_toClosedFork_isFork_aux_2 [simp]: 
+"increasing_tree F \<longrightarrow> increasing_tree (toClosedFork w F)"
+proof (induction F)
+  case Empty
+  then show ?case
+    by simp 
+next
+  case (Node n l)
+  then show ?case 
+      proof (cases "count_honest_node w (Node n l) = of_bool (isHonest w n)")
+        case True
+        then have "count_honest_node w (Node n l) = of_bool (isHonest w n)" by simp
+        then show ?thesis 
+          proof (cases "isHonest w n")
+            case True
+            then show ?thesis
+              by (metis \<open>count_honest_node w (Node n l) = of_bool (isHonest w n)\<close> 
+                 increasing_tree_branch_list_of_empty map_ListOfEmpty toClosedFork.simps(2)) 
+          next
+            case False
+            then show ?thesis
+              using True increasing_tree.simps(1) toClosedFork.simps(2) by presburger 
+          qed
+      next
+        case False
+        then have "toClosedFork w (Node n l) = Node n (map (toClosedFork w) l)"
+          by simp
+        have " (\<And>x2a. x2a \<in> set l \<Longrightarrow> increasing_tree x2a \<longrightarrow> increasing_tree (toClosedFork w x2a))"
+          using Node.IH by blast
+        have "increasing_tree (Node n l) \<longrightarrow> (\<forall>x \<in> set l. increasing_tree x \<and> lt_nat_tree n x)"
+          using increasing_tree_ind by blast 
+        then have "\<forall>x \<in> set l. lt_nat_tree n x \<longrightarrow> lt_nat_tree n (toClosedFork w x)"
+          by (metis (no_types, lifting) lt_nat_tree.simps(1) lt_nat_tree.simps(2) toClosedFork.elims) 
+        then show ?thesis
+          by (metis (mono_tags, lifting) Node.IH \<open>toClosedFork w (Node n l) = Node n (map (toClosedFork w) l)\<close> 
+imageE image_set increasing_tree_ind) 
+      qed
+qed
+
+lemma map_eq_map2 : "(\<forall> x \<in> set l. f x = f (g x)) \<longrightarrow> map f l = map f (map g l)"
+  by simp
+
+lemma honest_node_0_imp_0_each_honest_node : "count_honest_node w F = 0 \<longrightarrow> (\<forall> x \<in> H w. count_node x F = 0)"    
+  proof (induction F)
+    case Empty
+    then show ?case
+      using count_node.simps(1) by blast 
+  next
+    case (Node n l)
+    then show ?case
+      proof (cases "n \<in> H w")
+        case True
+          then have "count_honest_node w (Node n l) = (of_bool (n \<in> H w)) +  ListSum (map (count_node_by_set (H w)) l)"
+            using count_honest_node_def count_node_by_set.simps(2) by presburger
+          hence "count_honest_node w (Node n l) > 0"
+            by (metis True add_is_0 gr_zeroI of_bool_eq(1) of_bool_eq_iff)
+        then show ?thesis
+          by linarith 
+      next
+        case False
+          then have "count_honest_node w (Node n l) =  ListSum (map (count_node_by_set (H w)) l)"
+            by (metis (mono_tags, lifting) add.left_neutral count_honest_node_def count_node_by_set.simps(2) of_bool_eq(1))
+          hence "count_honest_node w (Node n l) = ListSum (map (count_honest_node w) l)"
+            by (metis count_honest_node_def map_eq_conv)
+          hence "count_honest_node w (Node n l) = 0 \<longrightarrow> (\<forall>x \<in> set l. count_honest_node w x = 0)"
+            by (metis (full_types) ListSum_0 image_eqI set_map)
+          hence "count_honest_node w (Node n l) = 0 \<longrightarrow> (\<forall>x \<in> set l. (\<forall>y \<in> H w. count_node y x = 0))"
+            using Node.IH by blast
+          then show ?thesis
+            by (smt False \<open>count_honest_node w (Node n l) = 0 \<longrightarrow> (\<forall>x\<in>set l. count_honest_node w x = 0)\<close> 
+\<open>count_honest_node w (Node n l) = ListSum (map (count_honest_node w) l)\<close> add_cancel_left_left count_node.elims map_eq_conv nattree.inject of_bool_eq(1))
+      qed
+  qed  
+  
+lemma isFork_toClosedFork_isFork_aux_3_aux [simp] :
+  assumes "isHonest w n" shows "count_node n F = count_node n (toClosedFork w F)" 
+proof (induction F)
+  case Empty
+  then show ?case
+    using toClosedFork.simps(1) by presburger 
+next
+  case (Node m l)
+  then show ?case
+    proof (cases "count_honest_node w (Node m l) = of_bool (isHonest w m)")
+      case True
+        then have "count_honest_node w (Node m l) = of_bool (isHonest w m)"
+          by simp
+        then show ?thesis 
+          proof (cases "isHonest w m")
+            case True
+            hence "isHonest w m"
+              by simp 
+            have "count_honest_node w (Node m l) = 1"
+              by (simp add: True \<open>count_honest_node w (Node m l) = of_bool (isHonest w m)\<close>) 
+            hence "count_honest_node w (toClosedFork w (Node m l)) =1"
+              by (smt Leaf.intros Leaf_non_ListOfEmpty ListSum_0 Listmax_ge One_nat_def Suc_eq_plus1_left 
+True count_honest_node_def count_node_by_set.simps(1) count_node_by_set.simps(2) isHonest_def le_0_eq 
+listmax_0 map_ListOfEmpty of_bool_eq(2) toClosedFork.simps(2))
+            hence ListSumhonest0 :"ListSum (map (count_honest_node w) l) = 0" 
+              by (smt One_nat_def Suc_eq_plus1_left True \<open>count_honest_node w (Node m l) = 1\<close> add_diff_cancel_left' count_honest_node_def count_node_by_set.simps(2) isHonest_def map_eq_conv of_bool_eq(2))
+            hence "\<forall>x \<in> set (map (count_honest_node w) l). x = 0"
+              using ListSum_0 by blast
+            hence "\<forall>x \<in> set l. count_honest_node w x = 0"
+              by simp
+            hence "\<forall>x \<in> set l. count_node n x = 0"
+              using assms honest_node_0_imp_0_each_honest_node isHonest_def by blast
+            hence "ListSum (map (count_node n) l) = 0"
+              by (metis ListSumhonest0 \<open>\<forall>x\<in>set l. count_honest_node w x = 0\<close> list.map_cong0 map_eq_map_tailrec)
+            hence "count_node n (Node m l) = of_bool (n = m)"
+              by (metis Leaf.intros ListMax_0 ListOfEmpty.simps ListSum_0 Listmax_ge Suc_le_eq \<open>ListSum (map (count_node n) l) = 0\<close> count_node.simps(2) count_node_Leaf gr0_conv_Suc gr_implies_not0 list.map_disc_iff not_gr0)
+            have "ListSum (map (count_honest_node w) (map (\<lambda>x. Empty) l)) = 0"
+              by (smt ListSum_0 count_honest_node_def count_node_by_set.simps(1) imageE set_map)
+            hence "count_node n (Node m (map (\<lambda>x. Empty) l)) = of_bool (n = m)"
+              using Leaf.simps count_node_Leaf map_ListOfEmpty by blast
+            then show ?thesis
+              using True \<open>count_honest_node w (Node m l) = of_bool (isHonest w m)\<close> \<open>count_node n (Node m l) = of_bool (n = m)\<close> by auto    
+          next
+            case False
+              hence "count_honest_node w (Node m l) = 0"
+                by (simp add: True)
+              hence "count_node n (Node m l) = 0"
+                using assms honest_node_0_imp_0_each_honest_node isHonest_def by blast 
+            then show ?thesis
+              by (simp add: False \<open>count_honest_node w (Node m l) = 0\<close>) 
+          qed
+    next
+      case False
+        have "toClosedFork w (Node m l) = Node m (map (toClosedFork w) l)"
+          by (simp add: False)
+        hence LHS:"count_node n (Node m l) = (of_bool (m = n)) + ListSum (map (count_node n) l)"
+          by auto
+        hence RHS:"count_node n (toClosedFork w (Node m l)) = (of_bool (m = n)) + ListSum (map (count_node n) (map (toClosedFork w) l))"
+          using \<open>toClosedFork w (Node m l) = Node m (map (toClosedFork w) l)\<close> by auto
+        have "\<forall>x \<in> set l. count_node n x = count_node n (toClosedFork w x)"
+          by (simp add: Node.IH)
+        hence "map (count_node n) l = map (count_node n) (map (toClosedFork w) l)"
+          using map_eq_map2 by blast
+      then show ?thesis using Node.IH LHS RHS by presburger
+    qed
+qed
+  
+lemma isFork_toClosedFork_isFork_aux_3 [simp]:
+  "uniqueH_tree F w \<longrightarrow> uniqueH_tree (toClosedFork w F) w"
+proof -
+  have "\<forall> x \<in> H w. count_node x F = count_node x (toClosedFork w F)"
+    using isFork_toClosedFork_isFork_aux_3_aux isHonest_def by blast
+  hence "uniqueH_tree F w \<longrightarrow> (\<forall>x \<in> H w. unique_node F x)"
+    using uniqueH_tree_def unique_nodes_by_nat_set.elims(2) by blast 
+  hence "uniqueH_tree F w \<longrightarrow> (\<forall>x \<in> H w. unique_node (toClosedFork w F) x)"
+    by (metis \<open>\<forall>x\<in>H w. count_node x F = count_node x (toClosedFork w F)\<close> unique_node_def)
+  thus ?thesis
+    using uniqueH_tree_in_imp_r by blast
+qed
+  
+lemma none_depth_imp_zero_exist [simp]: "depth F m = None \<longrightarrow> count_node m F = 0"
+proof (induction F)
+  case Empty
+  then show ?case
+    by simp 
+next
+  case (Node n l) 
+  hence depth:"depth (Node n l) m = (if n = m then (Some 0) else SucOption (ListMaxOption (map (\<lambda>x. depth x m) l)))"
+    using depth.simps(2) by blast 
+  hence "n = m \<longrightarrow> depth (Node n l) m = Some 0" by simp
+  have "depth (Node n l) m = None \<longrightarrow> n \<noteq> m" using depth
+    by fastforce 
+  hence "depth (Node n l) m = None \<longrightarrow> SucOption (ListMaxOption (map (\<lambda>x. depth x m) l)) = None"
+    by (metis depth)
+  hence "depth (Node n l) m = None \<longrightarrow> ListMaxOption (map (\<lambda>x. depth x m) l) = None"
+    using SucOption_none by blast
+  hence "depth (Node n l) m = None \<longrightarrow> (\<forall>x \<in> set l. depth x m = None)" by (metis ListMaxOption_none_imp_all_none image_eqI image_set) 
+  then show ?case
+    by (smt ListSum_0 Listmax_ge Node.IH \<open>depth (Node n l) m = None \<longrightarrow> n \<noteq> m\<close> add.left_neutral count_node.simps(2) le_0_eq listmax_0 of_bool_eq(1)) 
+qed
+
+lemma zero_exist_imp_none_depth [simp]: "count_node m F = 0 \<longrightarrow> depth F m = None" 
+proof (induction F)
+  case Empty
+  then show ?case
+    by simp 
+next
+  case (Node n l)
+    have "count_node m (Node n l) = 0 \<longrightarrow> n \<noteq> m \<and> ListSum (map (count_node m) l) = 0"
+      by simp
+    hence "count_node m (Node n l) = 0 \<longrightarrow> n \<noteq> m \<and> (\<forall>x \<in> set (map (count_node m) l). x = 0)"
+      using ListSum_0 by blast
+    hence "count_node m (Node n l) = 0 \<longrightarrow> n \<noteq> m \<and> (\<forall>x \<in> set l. count_node m x = 0)"
+      by (metis image_eqI set_map)
+    hence "count_node m (Node n l) = 0 \<longrightarrow> n \<noteq> m \<and> (\<forall>x \<in> set l. depth x m = None)"
+      using Node.IH by blast  
+  then show ?case
+    by (metis (no_types, lifting) ListMaxOption_none_imp_all_none SucOption_def depth.simps(2) imageE image_set option.case_eq_if) 
+qed
+  
+lemma isFork_toClosedFork_isFork_aux_4_aux [simp] : 
+  "isHonest w m \<longrightarrow> depth F m = depth (toClosedFork w F) m"
+proof (induction F)
+  case Empty
+  then show ?case
+    by simp 
+next
+  case (Node n l)
+  then show ?case 
+  proof (cases "count_honest_node w (Node n l) = of_bool (isHonest w n)")
+    case True
+      hence "count_honest_node w (Node n l) = of_bool (isHonest w n)" by simp
+      then show ?thesis 
+      proof (cases "isHonest w n")
+        case True
+          have "count_honest_node w (Node n l) = 1"
+            by (simp add: True \<open>count_honest_node w (Node n l) = of_bool (isHonest w n)\<close>)
+          have "ListSum (map (count_honest_node w) l) = 0"
+            by (smt One_nat_def Suc_eq_plus1_left True \<open>count_honest_node w (Node n l) = 1\<close> 
+add_diff_cancel_left' count_honest_node_def count_node_by_set.elims isHonest_def map_eq_conv nattree.distinct(1) nattree.inject of_bool_eq(2))
+          hence "\<forall>x \<in> set l. count_honest_node w x = 0"
+            by (metis (full_types) ListSum_0 image_eqI set_map)
+          hence "isHonest w m \<longrightarrow> (\<forall>x \<in> set l. count_node m x = 0)"
+           using honest_node_0_imp_0_each_honest_node isHonest_def by blast
+          hence "isHonest w m \<longrightarrow> count_node m (Node n l) = of_bool (m = n)"
+            by (metis \<open>ListSum (map (count_honest_node w) l) = 0\<close> \<open>\<forall>x\<in>set l. count_honest_node w x = 0\<close> 
+add_cancel_left_right count_node.simps(2) map_eq_conv)
+          hence "isHonest w m \<and> depth (Node n l) m \<noteq> None \<longrightarrow> count_node m (Node n l) \<noteq> 0"
+            by (meson zero_exist_imp_none_depth)
+          hence  "isHonest w m \<and> depth (Node n l) m \<noteq> None \<longrightarrow> m = n"
+            by (metis (full_types) \<open>isHonest w m \<longrightarrow> count_node m (Node n l) = of_bool (m = n)\<close> of_bool_eq(1))
+          hence L:"isHonest w m \<and> depth (Node n l) m \<noteq> None \<longrightarrow> depth (Node n l) m = Some 0"
+            by (meson depth.simps(2))
+          have "m = n \<longrightarrow> depth (Node n (map (\<lambda>x. Empty) l)) m = Some 0"   
+            by (meson depth.simps(2))
+          hence R:"isHonest w m \<and> depth (Node n l) m \<noteq> None \<longrightarrow> depth (toClosedFork w (Node n l)) m = Some 0"
+            using True
+            using \<open>count_honest_node w (Node n l) = 1\<close> \<open>isHonest w m \<and> depth (Node n l) m \<noteq> None \<longrightarrow> m = n\<close> by fastforce 
+          then show ?thesis using L R
+            by (metis (full_types) isFork_toClosedFork_isFork_aux_3_aux none_depth_imp_zero_exist zero_exist_imp_none_depth)
+      next
+        case False
+          have "count_honest_node w (Node n l) = 0"
+            by (simp add: False True)
+          hence "isHonest w m \<longrightarrow> count_node m (Node n l) = 0"
+            using honest_node_0_imp_0_each_honest_node isHonest_def by blast   
+          then show ?thesis
+            by (metis isFork_toClosedFork_isFork_aux_3_aux zero_exist_imp_none_depth) 
+      qed
+  next
+    case False
+      have "toClosedFork w (Node n l) = Node n (map (toClosedFork w) l)" using False
+        by simp
+      have "count_honest_node w (Node n l) \<noteq> of_bool (isHonest w n)"
+        by (simp add: False)
+      hence "ListSum (map (count_honest_node w) l) \<noteq> 0"
+        by (smt add.right_neutral count_honest_node_def count_node_by_set.simps(2) isHonest_def map_eq_conv)
+        (*isHonest w m \<and> depth (Node n l) m \<noteq> None \<longrightarrow> depth (Node n l) m = depth (toClosedFork w (Node n l)) m*)
+      then show ?thesis
+        by (metis (no_types, lifting) Node.IH \<open>toClosedFork w (Node n l) = Node n (map (toClosedFork w) l)\<close> depth.simps(2) map_eq_map2)         
+  qed
+qed
+    
+lemma isFork_toClosedFork_isFork_aux_4 [simp]: 
+ "increasing_depth_H F w \<longrightarrow> increasing_depth_H (toClosedFork w F) w"
+  by (smt increasing_depth_H.elims(2) increasing_depth_H.elims(3) isFork_toClosedFork_isFork_aux_4_aux isHonest_def)
+ 
+
+lemma isFork_toClosedFork_isFork_aux_5 [simp]:    
+  assumes "root_label_0 F" shows "root_label_0 (toClosedFork w F)"  
+proof -
+   obtain l where "F = Node 0 l"
+     using assms root_label_0.cases by blast
+   thus ?thesis
+   proof (cases "count_honest_node w (Node 0 l) = 1")
+     case True
+     hence "toClosedFork w F = Node 0 (map (\<lambda>x. Empty) l)"
+       by (metis (full_types) H_0 \<open>F = Node 0 l\<close> isHonest_def of_bool_eq(2) toClosedFork.simps(2))
+     then show ?thesis by (simp add: root_label_0.simps)
+   next
+     case False
+       hence "toClosedFork w F = Node 0 (map (toClosedFork w) l)"
+         by (metis (full_types) H_0 \<open>F = Node 0 l\<close> count_honest_node_def count_node_by_set.simps(2)
+ le_add_same_cancel1 not_one_le_zero of_bool_eq(1) of_bool_eq(2) toClosedFork.simps(2) zero_le)
+     then show ?thesis
+       by (simp add: root_label_0.simps) 
+   qed
+qed
+  
 lemma isFork_toClosedFork_isFork [simp]: "isFork w F \<longrightarrow> isFork w (toClosedFork w F)"
-  sorry
-    
-lemma closedFork_eq_toClosedFork [simp]: "isFork w F \<longrightarrow> F = (toClosedFork w F)"
-  sorry 
+  using isFork.simps isFork_toClosedFork_isFork_aux_1 isFork_toClosedFork_isFork_aux_2 
+isFork_toClosedFork_isFork_aux_3 isFork_toClosedFork_isFork_aux_4 isFork_toClosedFork_isFork_aux_5 by blast
+  
+lemma foldr_conj_eq_forall [simp]: "foldr conj l True \<longleftrightarrow> (\<forall> x \<in> set l. x)"    
+  proof (induction l)
+    case Nil
+    then show ?case
+      by auto 
+  next
+    case (Cons x xs)
+    hence "foldr conj (x#xs) True = (x \<and> foldr conj xs True)"
+      by auto
+    then show ?case
+      using Cons.IH by auto 
+  qed
+  
+lemma toClosedFork_closedFork_aux [simp]: "(closedFork_Hgiven (toClosedFork w F) (H w))"  
+proof (induction F)
+  case Empty
+  then show ?case
+    using closedFork_Hgiven.simps(1) toClosedFork.simps(1) by presburger 
+next
+  case (Node n l)
+     hence "\<forall>x \<in> set l. closedFork_Hgiven (toClosedFork w x) (H w)"
+       by blast 
+     hence "\<forall>x \<in> set (map (toClosedFork w) l). closedFork_Hgiven x (H w)"
+       by (metis (mono_tags, hide_lams) imageE set_map)
+     hence "\<forall>x \<in> set (map (toClosedFork w) l). (\<lambda>x. closedFork_Hgiven x (H w)) x"
+       by blast
+     hence f1: "\<forall>x \<in> set (map (\<lambda>x. closedFork_Hgiven x (H w)) (map (toClosedFork w) l)). x"
+       by (metis (no_types, lifting) image_iff list.set_map)
+  then show ?case 
+    proof (cases "count_honest_node w (Node n l) = of_bool (isHonest w n)")
+      case True
+        hence "count_honest_node w (Node n l) = of_bool (isHonest w n)" by simp
+      then show ?thesis 
+        proof (cases "isHonest w n")
+          case True
+            hence "toClosedFork w (Node n l) = Node n (map (\<lambda>x. Empty) l)"
+              by (simp add: \<open>count_honest_node w (Node n l) = of_bool (isHonest w n)\<close>)
+          then show ?thesis
+            by (metis True closedFork_Hgiven.simps(2) isHonest_def map_ListOfEmpty) 
+        next
+          case False
+          then show ?thesis
+            using True closedFork_Hgiven.simps(1) toClosedFork.simps(2) by presburger    
+        qed
+    next
+      case False
+        hence "toClosedFork w (Node n l) = Node n (map (toClosedFork w) l)"
+          by simp
+        hence f2:"closedFork_Hgiven (toClosedFork w (Node n l)) (H w) = (if ListOfEmpty (map (toClosedFork w) l) 
+                                                                      then (n \<in> (H w)) 
+                                                                      else foldr conj (map (\<lambda>x. closedFork_Hgiven x (H w)) (map (toClosedFork w) l)) True)"
+          using closedFork_Hgiven.simps(2) by presburger
+        have "ListSum (map (count_node_by_set (H w)) l) > 0" using False
+          by (simp add: H_def count_honest_node_def isHonest_def)
+        obtain child where "child \<in> set l \<and> count_node_by_set (H w) child > 0"
+          by (metis ListSum_0 Listmax_ge \<open>0 < ListSum (map (count_node_by_set (H w)) l)\<close> le_zero_eq listmax_0 neq0_conv)
+        obtain m bl where "child = Node m bl"
+          by (metis \<open>child \<in> set l \<and> 0 < count_node_by_set (H w) child\<close> count_node_by_set.elims neq0_conv)
+        hence "toClosedFork w (Node m bl) \<noteq> Empty" 
+          proof -
+           have "0 < count_honest_node w child"
+            using \<open>child \<in> set l \<and> 0 < count_node_by_set (H w) child\<close> count_honest_node_def by presburger
+           then show ?thesis
+             by (simp add: \<open>child = Node m bl\<close>)
+         qed
+        hence "\<not> ListOfEmpty (map (toClosedFork w) l)"
+          by (metis Leaf.intros Leaf_non_ListOfEmpty \<open>child = Node m bl\<close> \<open>child \<in> set l \<and> 0 < count_node_by_set (H w) child\<close> image_eqI set_map)
+        hence "closedFork_Hgiven (toClosedFork w (Node n l)) (H w) = foldr conj (map (\<lambda>x. closedFork_Hgiven x (H w)) (map (toClosedFork w) l)) True"
+          using f2 by presburger
+        then show ?thesis using f1 foldr_conj_eq_forall
+          by blast
+    qed
+qed
 
-lemma toClosedFork_prefixFork [simp]: "isFork w F \<longrightarrow> isPrefix_fork w w F (toClosedFork w F)"
-  sorry
+lemma toClosedFork_closedFork [simp]: "isFork w F \<longrightarrow> closedFork (toClosedFork w F) w"  
+proof (cases F)
+  case Empty
+  then show ?thesis
+    using closedFork_Hgiven.simps(1) closedFork_def toClosedFork.simps(1) by presburger 
+next
+  case (Node n l)
+    then show ?thesis
+      using closedFork_def isFork_toClosedFork_isFork toClosedFork_closedFork_aux by blast 
+qed
+   
+lemma length_langest_tine_eq_height_aux_0 [simp]: "x \<in> set_of_tines F \<longrightarrow> length x \<le> height F"
+  by simp
+  
+lemma length_langest_tine_eq_height_aux_1 [simp]: "\<exists> x \<in> set_of_tines F. length x = height F"
+ proof (induction F)
+   case Empty
+   then show ?case by simp
+ next
+   case (Node n l)
+   then show ?case
+     proof (cases "Leaf (Node n l)")
+       case True
+       then show ?thesis
+         by (metis height.simps(2) list.size(3) nil_in_set_of_tines) 
+     next
+       case False
+        hence "height (Node n l) = Suc (ListMax (map height l))"
+          by (meson height.simps(2))
+        obtain y where "y \<in> set (map height l) \<and> y = ListMax (map height l)"
+          by (metis False Leaf.intros ListMax_member ListOfEmpty.Nil list.map_disc_iff)
+        then obtain a where "a \<in> set l \<and> a \<noteq> Empty \<and> height a = ListMax (map height l)"
+          by (metis (no_types, lifting) False Leaf_non_ListOfEmpty Listmax_ge height.simps(1) imageE image_eqI le_0_eq set_map)
+        then obtain b where "b \<in> set_of_tines a \<and> length b = height a"
+          using Node.IH by blast
+        then obtain m where "m < length l \<and> nth l m = a"
+          by (meson \<open>a \<in> set l \<and> a \<noteq> Empty \<and> height a = ListMax (map height l)\<close> in_set_conv_nth)
+        then obtain nn ll where "a = Node nn ll"
+          using \<open>a \<in> set l \<and> a \<noteq> Empty \<and> height a = ListMax (map height l)\<close> max_node.cases by blast
+        then have "getLabelFromTine (Node n l) (m#b) = nn#(getLabelFromTine a b)"
+          by (metis \<open>m < length l \<and> l ! m = a\<close> getLabelFromTine.simps(3) nattree.simps(5) not_less)
+          then show ?thesis
+            by (metis \<open>a \<in> set l \<and> a \<noteq> Empty \<and> height a = ListMax (map height l)\<close> \<open>b \<in> set_of_tines a \<and> length b = height a\<close> \<open>height (Node n l) = Suc (ListMax (map height l))\<close> \<open>m < length l \<and> l ! m = a\<close> getLabelFromTine_branch_in_if length_Cons) 
+         
+     qed
+ qed
     
-lemma closedFork_deepest_honest_node_eq_height [simp]: "isFork w F \<and> closedFork F w \<longrightarrow> 
-          depth (ClosedFork w F) (max_honest_node w) = Some (height F)"
-  sorry
+lemma length_langest_tine_eq_height [simp]: "(\<forall>x \<in> set_of_tines F. length x \<le> height F) \<and> (\<exists>x \<in> set_of_tines F. length x = height F)"
+  using length_langest_tine_eq_height_aux_1 by auto
+  
+lemma exist_Some_eq_ListMaxOption_ne_None [simp]: "(\<exists>x. Some x \<in> set l) \<longleftrightarrow> ListMaxOption l \<noteq> None"
+  by auto     
     
-lemma obtain_two_non_negative_reach_tines_toClosedFork [simp]: 
-  assumes "isFork w F \<and> flatFork w F" 
-  shows "t1 \<in> set (tinelist F) \<and> t2 \<in> set (tinelist F) 
-\<and> length t1 = length t2 \<and> length t1 = height F 
+lemma ListMaxOption_Max_Some [simp]: "ListMaxOption l = None \<or> (\<exists>x. ListMaxOption l = Some x \<and> Some x \<in> set l \<and> (\<forall>y. Some y \<in> set l \<longrightarrow> y \<le> x))"
+  proof (induction l)
+    case Nil
+    then show ?case by simp
+  next
+    case (Cons x xs)
+    then show ?case 
+      proof (cases x)
+        case None
+          have "ListMaxOption (None#xs) = ListMaxOption xs"
+            by (simp add: ListMaxOption_def)
+        then show ?thesis
+          by (metis Cons.IH None insert_iff list.simps(15) option.distinct(1))
+      next
+        case (Some M)
+          hence "x = Some M"
+            by simp
+        then show ?thesis 
+          proof (cases "ListMaxOption xs")
+            case None
+              hence "ListMaxOption (x#xs) = Some M"
+                by (simp add: ListMaxOption_def Some)
+            then show ?thesis
+              by (metis None Some eq_iff exist_Some_eq_ListMaxOption_ne_None option.inject set_ConsD) 
+          next
+            case (Some a)
+            then show ?thesis 
+              proof (cases "a < M")
+                case True
+                hence "ListMaxOption (x#xs) = Some M"
+                  using ListMaxOption_def Some \<open>x = Some M\<close> by auto
+                then show ?thesis
+                  using Cons.IH Some True \<open>x = Some M\<close> by auto 
+              next
+                case False
+                  hence "ListMaxOption (x#xs) = Some a"
+                  using ListMaxOption_def Some \<open>x = Some M\<close> by auto
+                then show ?thesis
+                  using Cons.IH Some False \<open>x = Some M\<close> by auto 
+          qed
+      qed
+  qed
+qed
+  
+lemma depth_le_height [simp]: "count_node x F = 0 \<or> le_option (depth F x) (Some (height F))"    
+ proof (induction F)
+ case Empty
+   then show ?case
+    by simp 
+ next
+   case (Node n l)
+   then show ?case 
+     proof (cases "count_node x (Node n l) = 0")
+       case True
+       then show ?thesis by blast
+     next
+       case False
+         hence "count_node x (Node n l) \<noteq> 0"
+           by simp
+         have "\<forall>y \<in> set l. count_node x y = 0 \<or> le_option (depth y x) (Some (height y))"
+           using Node.IH by blast
+         have "\<forall>y \<in> set l. count_node x y = 0 \<longrightarrow> depth y x = None"
+           using zero_exist_imp_none_depth by blast
+         hence "\<forall>y \<in> set l. count_node x y = 0 \<longrightarrow> \<not> le_option (depth y x) (Some (height y))"
+           by (metis le_option.cases option.simps(3))
+         hence f1:"depth (Node n l) x = (if n = x 
+                          then (Some 0) 
+                          else SucOption (ListMaxOption (map (\<lambda>y. depth y x) l)))"
+           using depth.simps(2) by blast
+         then show ?thesis 
+           proof (cases "n=x")
+             case True
+             then show ?thesis
+               using \<open>depth (Node n l) x = (if n = x then Some 0 else SucOption (ListMaxOption (map (\<lambda>y. depth y x) l)))\<close> le0 le_option.intros by presburger 
+           next
+             case False
+               then obtain w where w:"(ListMaxOption (map (\<lambda>y. depth y x) l)) = Some w \<and> Some w \<in> set (map (\<lambda>y. depth y x) l)"
+                 by (metis (no_types, lifting) False ListMaxOption_Max_Some SucOption_def 
+\<open>count_node x (Node n l) \<noteq> 0\<close> f1 none_depth_imp_zero_exist option.simps(4))
+               then obtain y where "y \<in> set l \<and> depth y x = Some w"
+                 by (metis imageE set_map)    
+               have "depth (Node n l) x = Some (Suc w)" using w
+                 by (metis False SucOption_def \<open>depth (Node n l) x = (if n = x then Some 0 else 
+SucOption (ListMaxOption (map (\<lambda>y. depth y x) l)))\<close> option.simps(5))
+               have "le_option (depth y x) (Some (height y))"
+                 by (metis Node.IH \<open>\<forall>y\<in>set l. count_node x y = 0 \<longrightarrow> depth y x = None\<close> \<open>y \<in> set l \<and> depth y x = Some w\<close> option.distinct(1))
+               hence "w \<le> height y"
+                 by (metis \<open>y \<in> set l \<and> depth y x = Some w\<close> le_option.cases option.inject)
+               hence "Suc (height y) \<le> height (Node n l)"
+                 by (metis Leaf_non_ListOfEmpty Listmax_ge \<open>\<forall>y\<in>set l. count_node x y = 0 \<longrightarrow> 
+\<not> le_option (depth y x) (Some (height y))\<close> \<open>le_option (depth y x) (Some (height y))\<close> \<open>y \<in> set l \<and> 
+depth y x = Some w\<close> count_node.simps(1) height.simps(2) image_eqI not_less_eq_eq set_map)
+               then show ?thesis
+                 by (metis \<open>depth (Node n l) x = Some (Suc w)\<close> \<open>w \<le> height y\<close> le_option.intros le_trans not_less_eq_eq) 
+           qed           
+     qed
+ qed
+
+fun max_exist_honest_node :: "nattree \<Rightarrow> bool list \<Rightarrow> nat" where
+  "max_exist_honest_node Empty _ = 0"
+| "max_exist_honest_node (Node n l) w = 
+(if isHonest w n 
+then max n (ListMax (map (\<lambda>x. max_exist_honest_node x w) l)) 
+else ListMax (map (\<lambda>x. max_exist_honest_node x w) l))"    
+
+lemma  exist_le_real_max [simp]: "max_exist_honest_node F w \<le> max_honest_node w" 
+proof (induction F)
+  case Empty
+  then show ?case
+    by simp
+next
+  case (Node n l)
+    hence f1:"max_exist_honest_node (Node n l) w = (if isHonest w n 
+then max n (ListMax (map (\<lambda>x. max_exist_honest_node x w) l)) 
+else ListMax (map (\<lambda>x. max_exist_honest_node x w) l))"
+      by simp 
+    have f2:"ListMax (map (\<lambda>x. max_exist_honest_node x w) l) \<le> max_honest_node w"
+      by (metis (no_types, lifting) ListMax_member Node gr_implies_not_zero imageE leI list.map_disc_iff 
+listmax_0 max_exist_honest_node.simps(1) set_map)
+  have f3 :"isHonest w n \<longrightarrow> n \<le> max_honest_node w"
+    by (metis Sup_fin.bounded_iff Sup_fin_Max equals0D finite_honest_node isHonest_def le_refl max_honest_node_def)
+  then show ?case using f1 f2 f3 by simp
+qed
+    
+lemma isFork_max_exist_honest_node_eq_max_honest_node [simp]: 
+"count_node (max_honest_node w) F \<noteq> 0 \<longrightarrow> max_exist_honest_node F w = max_honest_node w" 
+proof (induction F) 
+  case Empty 
+  then show ?case 
+    by simp 
+next
+  case (Node n l)
+  then show ?case 
+  proof (cases "(max_honest_node w) = n")
+    case True
+      hence "count_node (max_honest_node w) (Node n l) > 0"
+        by simp
+      hence f1:"max_exist_honest_node (Node n l) w = (if isHonest w n 
+then max n (ListMax (map (\<lambda>x. max_exist_honest_node x w) l)) 
+else ListMax (map (\<lambda>x. max_exist_honest_node x w) l)) "
+        by simp
+      have "isHonest w n" using True
+        by (metis H_0 Max_in equals0D finite_honest_node isHonest_def max_honest_node_def)
+      hence "max_exist_honest_node (Node n l) w = max n (ListMax (map (\<lambda>x. max_exist_honest_node x w) l))"
+        using f1 by simp
+    then show ?thesis
+      by (metis True exist_le_real_max max.commute max_def) 
+  next
+    case False
+      hence unfold:"max_exist_honest_node (Node n l) w = (if isHonest w n 
+then max n (ListMax (map (\<lambda>x. max_exist_honest_node x w) l)) 
+else ListMax (map (\<lambda>x. max_exist_honest_node x w) l)) " by simp
+      have if_lt:"isHonest w n \<longrightarrow> n < max_honest_node w"
+      proof -
+        { assume "\<not> n \<le> 0"
+          { assume "\<not> n \<le> \<Squnion>\<^sub>f\<^sub>i\<^sub>n{n. n \<le> length w \<and> \<not> (False # w) ! n} \<and> \<not> n \<le> 0"
+            then have "max_exist_honest_node (Node n []) w \<noteq> max n 0"
+              by (metis H_def Sup_fin_Max exist_le_real_max max_def max_honest_node_def)
+            then have ?thesis
+              by auto }
+          then have "n \<le> \<Squnion>\<^sub>f\<^sub>i\<^sub>n{n. n \<le> length w \<and> \<not> (False # w) ! n} \<or> (isHonest w n \<longrightarrow> n < max_honest_node w)"
+            by blast }
+        then have "n \<le> \<Squnion>\<^sub>f\<^sub>i\<^sub>n{n. n \<le> length w \<and> \<not> (False # w) ! n} \<or> n < \<Squnion>\<^sub>f\<^sub>i\<^sub>n{n. n \<le> length w \<and> \<not> (False # w) ! n} \<or> (isHonest w n \<longrightarrow> n < max_honest_node w)"
+          by blast
+        then show ?thesis
+          by (metis False H_def Sup_fin_Max le_neq_implies_less max_honest_node_def)
+      qed
+      hence "count_node (max_honest_node w) (Node n l) \<noteq> 0 \<longrightarrow> ListSum (map (count_node (max_honest_node w)) l) \<noteq> 0"
+        using False by simp
+      hence f1:"count_node (max_honest_node w) (Node n l) \<noteq> 0 \<longrightarrow> (\<exists>x \<in> set l. count_node (max_honest_node w) x \<noteq> 0)"
+        by (metis ListSum_0 imageE image_set)
+      hence f2:"count_node (max_honest_node w) (Node n l) \<noteq> 0 \<longrightarrow> (\<exists>x \<in> set l. max_exist_honest_node x w = max_honest_node w)"
+        using Node.IH by blast
+      hence f3: "count_node (max_honest_node w) (Node n l) \<noteq> 0 \<longrightarrow> (\<exists>x \<in> set (map (\<lambda>y. max_exist_honest_node y w) l). x = max_honest_node w)"
+        by (metis (full_types) image_eqI set_map)
+      hence f4:"count_node (max_honest_node w) (Node n l) \<noteq> 0 \<longrightarrow> (\<forall>x \<in> set (map (\<lambda>y. max_exist_honest_node y w) l). x \<le> max_honest_node w)"
+        by simp
+      hence f5:"count_node (max_honest_node w) (Node n l) \<noteq> 0 \<longrightarrow> max_honest_node w \<le> ListMax (map (\<lambda>x. max_exist_honest_node x w) l)" using f1 f2
+         Listmax_ge f3 by blast
+      hence "count_node (max_honest_node w) (Node n l) \<noteq> 0 \<longrightarrow> ListMax (map (\<lambda>x. max_exist_honest_node x w) l) \<le> max_honest_node w" using f4 ListMax_member
+        by (metis ListMax_0 le0)
+    then show ?thesis using f5 if_lt
+      by fastforce
+  qed
+qed
+
+definition H_tree_and_string :: "nattree \<Rightarrow> bool list \<Rightarrow> nat set" where
+  "H_tree_and_string t w= {x. x \<in> H w \<and> count_node x t > 0}"
+
+definition uniqueH_nodes_in_tree :: "nattree \<Rightarrow> bool list \<Rightarrow> bool" where
+  "uniqueH_nodes_in_tree t l =(\<forall>x \<in> H l. count_node x t \<le> 1)"
+   
+lemma ind_uniqueH_nodes_in_tree [simp]: 
+"uniqueH_nodes_in_tree (Node n l) w \<longrightarrow> (\<forall>x \<in> set l. uniqueH_nodes_in_tree x w)"
+proof -
+  have "uniqueH_nodes_in_tree (Node n l) w = (\<forall>x \<in> H w. count_node x (Node n l) \<le> 1)"
+    using uniqueH_nodes_in_tree_def by blast
+  hence "uniqueH_nodes_in_tree (Node n l) w = (\<forall>x \<in> H w. (of_bool (n = x)) + ListSum (map (count_node x) l) \<le> 1)"
+    by (smt count_node.simps(2))
+  hence "uniqueH_nodes_in_tree (Node n l) w \<longrightarrow> (\<forall>x \<in> H w. ListSum (map (count_node x) l) \<le> 1)"
+    using le_add2 le_trans by blast
+  hence "uniqueH_nodes_in_tree (Node n l) w \<longrightarrow> (\<forall>x \<in> H w. \<forall>y \<in> set l. count_node x y \<le> 1)"
+    by (metis (no_types, lifting) ListSum_ge dual_order.trans image_eqI image_set)
+  then show ?thesis
+    using uniqueH_nodes_in_tree_def by blast
+qed   
+
+lemma ind_increasing_depth_H_tree_string_aux [simp]:    
+"(uniqueH_nodes_in_tree (Node n l) w) \<and> (\<forall> x \<in> (H_tree_and_string (Node n l) w. ) \<and> 
 \<longrightarrow> 
-(\<exists> t1' \<in> set (tinelist (toClosedFork w F)). 
-\<exists> t2' \<in> set (tinelist (toClosedFork w F)). 
-isPrefix_tine (toClosedFork w F) F t1' t1 
-\<and> isPrefix_tine (toClosedFork w F) F t2' t2
-\<and> edge_disjoint_tines t1' t2' 
-\<and> reach (toClosedFork w F) w t1' \<ge> 0 
-\<and> reach (toClosedFork w F) w t2' \<ge> 0)"  
+(\<forall> z \<in> set l . (uniqueH_nodes_in_tree z w) \<and> (\<forall> x y. x \<in> (H_tree_and_string z w) \<and> y \<in> (H_tree_and_string z w) \<and> x < y \<longrightarrow> lt_option (depth z x) (depth z y)))"
+  
+lemma ind_increasing_depth_H_tree_string [simp]: 
+"(uniqueH_nodes_in_tree (Node n l) w) \<and> (\<forall> x y. x \<in> (H_tree_and_string (Node n l) w) \<and> y \<in> (H_tree_and_string (Node n l) w) \<and> x < y 
+\<longrightarrow> lt_option (depth (Node n l) x) (depth (Node n l) y)) \<longrightarrow> 
+(\<forall> z \<in> set l . (uniqueH_nodes_in_tree z w) \<and> (\<forall> x y. x \<in> (H_tree_and_string z w) \<and> y \<in> (H_tree_and_string z w) \<and> x < y \<longrightarrow> lt_option (depth z x) (depth z y)))"  
+proof -
+  have "uniqueH_nodes_in_tree (Node n l) w \<longrightarrow> (\<forall>x \<in> set l. uniqueH_nodes_in_tree x w)" by simp
+  hence "uniqueH_nodes_in_tree (Node n l) w \<and> isHonest w n \<longrightarrow> count_node n (Node n l) = 1 \<and> ListSum (map (count_node n) l) = 0"
+    by (smt add_diff_cancel_left' count_node.simps(2) diff_is_0_eq eq_iff isHonest_def le_add1 of_bool_eq(2) uniqueH_nodes_in_tree_def)
+  
+     
+lemma colsedFork_height_eq_depth_max_honest_aux [simp]: 
+"closedFork_Hgiven F (H w) \<and> (uniqueH_nodes_in_tree F w) \<and>
+(\<forall> x y. x \<in> (H_tree_and_string F w) \<and> y \<in> (H_tree_and_string F w) \<and> x < y \<longrightarrow> lt_option (depth F x) (depth F y)) 
+\<longrightarrow> (Some (height F) = depth F (max_exist_honest_node F w) \<or> F = Empty)"
+sorry
+
+lemma closedFork_height_eq_depth_max_honest [simp]: "closedFork F w \<longrightarrow> Some (height F) = depth F (max_honest_node w)"
+proof (cases F)
+  case Empty
+  then show ?thesis
+    by (metis closedFork_def depth.simps(1) isFork.simps option.discI root_label_0_depth_0) 
+next
+  case (Node n l)
+  hence f0:"closedFork (Node n l) w \<longrightarrow> (isFork w (Node n l) \<and> closedFork_Hgiven (Node n l) (H w))"
+    using closedFork_def by blast
+  hence f1:"closedFork (Node n l) w \<longrightarrow> (isFork w (Node n l) \<and> closedFork_Hgiven (Node n l) (H_tree_and_string (Node n l) w))"
+    by (smt Collect_cong H_def H_tree_and_string_def gr0I isFork_uniqueH_tree mem_Collect_eq of_bool_eq(1) of_bool_eq(2) of_bool_eq_iff unique_node_def)
+  hence f2:"closedFork (Node n l) w \<longrightarrow> (uniqueH_nodes_in_tree (Node n l) w)"
+    by (metis isFork_uniqueH_tree less_or_eq_imp_le uniqueH_nodes_in_tree_def unique_node_def)    
+  have f3:"closedFork (Node n l) w \<longrightarrow> (uniqueH_tree (Node n l) w \<and> increasing_depth_H (Node n l) w \<and> closedFork_Hgiven (Node n l) (H_tree_and_string (Node n l) w))"
+    using f1 isFork.simps by blast
+  hence "closedFork (Node n l) w \<longrightarrow>  closedFork_Hgiven (Node n l) (H_tree_and_string (Node n l) w) \<and> 
+(\<forall> x y. x \<in> (H_tree_and_string (Node n l) w) \<and> y \<in> (H_tree_and_string (Node n l) w) \<and> x < y \<longrightarrow> lt_option (depth (Node n l) x) (depth (Node n l) y))"
+    by (metis (no_types, lifting) H_tree_and_string_def increasing_depth_H.simps mem_Collect_eq)
+  then show ?thesis
+    by (metis H_0 Max_in Node f2 f3 closedFork_def colsedFork_height_eq_depth_max_honest_aux equals0D 
+finite_honest_node isFork_max_exist_honest_node_eq_max_honest_node max_honest_node_def nattree.simps(3) 
+uniqueH_tree_def unique_node_def unique_nodes_by_nat_set.elims(2) zero_neq_one)
+qed 
+ 
+lemma closedFork_longest_tine_end_max_honest [simp]: "closedFork F w \<longrightarrow> 
+(\<exists>x \<in> set_of_tines F. Some (length x) = depth F (max_honest_node w) \<and> (\<forall>y \<in> set_of_tines F - {x}. length y < length x))"
   sorry
+    
+(*trying to find the way to describe the longest honest prefix 
+then use it to show that after the last node there are only adversarial ones
+and the length of original one is greater than or equal to the height now
+so the number of suffix adversarial nodes is greater than the different of the gap
+
+*)
+    
+lemma exist_longest_honest_prefix_tine [simp]: 
+"t \<in> set_of_tines F \<and> t \<noteq> [] \<and> isFork w F\<longrightarrow> 
+(\<exists>x. (isPrefix_tine F F t x) \<and> isHonest w (last x) \<and> (\<forall>y. isPrefix_tine F F t y \<and> isHonest w (last y) \<longrightarrow> length y < length x))"  
+  sorry
+  
+lemma toClosedFork_prefixFork [simp]: "isFork w F \<longrightarrow> isPrefix_fork w w F (toClosedFork w F)"
+  sorry   
+    
+lemma closedFork_deepest_honest_node_eq_height [simp]: "closedFork F w \<longrightarrow> 
+depth (ClosedFork w F) (max_honest_node w) = Some (height F)"
+  sorry
+    
+definition honestTine :: "nattree \<Rightarrow> bool list \<Rightarrow> nat list \<Rightarrow> bool" where
+  "honestTine t w tine = ((tine \<in> set_of_tines t) \<and> (getLabelFromTine t tine = [] \<or> isHonest w (last (getLabelFromTine t tine))))"
+
+lemma toClosedFork_honest_tines_biggest [simp]: 
+"isFork w F \<longrightarrow> (\<forall>tine \<in> set_of_tines F. honestTine F w tine \<longrightarrow> tine \<in> set_of_tines (toClosedFork w F))"    
+  sorry
+   
+lemma toClosedFork_height_le [simp]: 
+"height (toClosedFork w F) \<le> height F"
+  sorry 
+   
+lemma obtain_two_non_negative_reach_tines_toClosedFork [simp]: 
+  assumes "isFork w F" and "flatFork w F" and "\<not> ListOfAdverse w" 
+  shows "(\<exists> (t1,t2) \<in> set_of_edge_disjoint_tines (toClosedFork w F).
+reach (toClosedFork w F) w t1 \<ge> 0 
+\<and> reach (toClosedFork w F) w t2 \<ge> 0)"  
+proof -
+  have "closedFork (toClosedFork w F) w"
+    using assms(1) toClosedFork_closedFork by blast
+  have "(\<exists> t1 \<in> set_of_tines F.  \<exists> t2 \<in> set_of_tines F. 
+ length t1 = length t2 \<and> length t1 = height F \<and> edge_disjoint_tines t1 t1)"
+    by (meson assms(2) flatFork_def flatTree.elims(2)) 
+ show ?thesis    
+ sorry
+qed
+  
+lemma min_reach_image [simp]: "(\<lambda>x. min (reach F' w (fst x)) (reach F' w (snd x)))`(set_of_edge_disjoint_tines F') 
+= {r. (\<exists> (a,b) \<in> set_of_edge_disjoint_tines F'. r = min (reach F' w a) (reach F' w b))}"
+  by (smt Collect_cong case_prod_unfold image_def)
+  
   
 lemma if_4_17 [simp]: assumes "isForkable w" shows  "(\<exists> F.(isFork w F \<and> margin F w \<ge> 0))"
 proof (cases "ListOfAdverse w")
@@ -770,7 +1931,25 @@ proof (cases "ListOfAdverse w")
     using margin_no_honest by blast 
 next
   case False
-  then show ?thesis sorry
+  obtain F where F:"isFork w F \<and> flatFork w F"
+    using assms flatFork_def isForkable_def by blast 
+  then obtain F' where "F' = toClosedFork w F"
+    by blast
+  then obtain t1 and t2 where "(t1,t2) \<in> set_of_edge_disjoint_tines F' \<and> reach F' w t1 \<ge> 0 \<and> reach F' w t2 \<ge> 0" 
+    using F False obtain_two_non_negative_reach_tines_toClosedFork by blast
+  hence ge_0:"min (reach F' w t1) (reach F' w t2) \<ge> 0" by simp
+  hence isin:"min (reach F' w t1) (reach F' w t2) \<in> {r. (\<exists> (a,b) \<in> set_of_edge_disjoint_tines F'. r = min (reach F' w a) (reach F' w b))}"
+    using \<open>(t1, t2) \<in> set_of_edge_disjoint_tines F' \<and> 0 \<le> reach F' w t1 \<and> 0 \<le> reach F' w t2\<close> by auto
+  have "(\<lambda>x. min (reach F' w (fst x)) (reach F' w (snd x)))`(set_of_edge_disjoint_tines F') 
+= {r. (\<exists> (a,b) \<in> set_of_edge_disjoint_tines F'. r = min (reach F' w a) (reach F' w b))}" 
+    by (smt Collect_cong case_prod_unfold image_def)
+  hence finite: "finite {r. (\<exists> (a,b) \<in> set_of_edge_disjoint_tines F'. r = min (reach F' w a) (reach F' w b))}"
+    using set_of_edge_disjoint_tines_finite by auto
+  hence "Max {r. (\<exists> (a,b) \<in> set_of_edge_disjoint_tines F'. r = min (reach F' w a) (reach F' w b))} \<ge> min (reach F' w t1) (reach F' w t2) " using isin
+    by (simp add: isin)
+  hence "margin F' w \<ge> min (reach F' w t1) (reach F' w t2)" using margin_def by simp
+  then show ?thesis using ge_0 F
+    by (smt \<open>F' = toClosedFork w F\<close> isFork_toClosedFork_isFork) 
 qed
    
 lemma only_if_4_17 [simp]: assumes  "(\<exists> F.(isFork w F \<and> margin F w \<ge> 0))" shows " isForkable w"
@@ -836,7 +2015,7 @@ proof -
     then have "set_of_tines F = {tine. length tine = 0}"
       by (metis (no_types, lifting) Collect_cong list.size(3) set_of_tines.elims)
     then have set_nil:"set_of_tines F = {[]}"
-      by (smt Collect_cong length_greater_0_conv list.size(3) singleton_conv)
+      by auto
     then have "(\<forall> x \<in> set_of_tines F. reach F [] x = 0)"
       using f1 by (metis \<open>reach F [] [] = 0\<close> singletonD)
     have "(\<exists> x \<in> set_of_tines F. reach F [] x = 0)"
@@ -934,7 +2113,8 @@ lemma lemma_4_18_trivial_case_m : "m [] = (0,0)"
 
 lemma lemma_4_18_trivial_case_exist_Fork : 
 "\<exists> F. (isFork [] F \<and> closedFork F []  \<and> (m [] = (lambda F [], margin F [])))"
-  by (metis ListOfAdverse.Nil closedFork_ListOfAdverse isFork_Nil lambda_of_nil_aux lemma_4_18_trivial_case_m margin_no_honest margin_of_nil_aux root_label_0.cases)
+  by (metis ListOfAdverse.Nil closedFork_ListOfAdverse isFork_Nil lambda_of_nil_aux                  
+lemma_4_18_trivial_case_m margin_no_honest margin_of_nil_aux root_label_0.cases)
   
 lemma lemma_4_18 : "(m [] = (0,0)) \<and> 
   (\<forall> w. ((length w > 0) \<longrightarrow> ( 
@@ -945,6 +2125,5 @@ lemma lemma_4_18 : "(m [] = (0,0)) \<and>
      \<and>   (lambda_of_string w > 0 \<and> margin_of_string w \<noteq> 0 \<longrightarrow> (m (w @ [False]) 
           = (lambda_of_string w - 1, margin_of_string w - 1))))) 
 \<and> (\<exists> F. (isFork w F \<and> closedFork F w  \<and> (m w = (lambda F w, margin F w)))))"
-  sorry
-    
+  sorry 
 end
